Rename mod_step to io_step

gol_io_stepScript.sml
@@ -6,7 +6,7 @@ open pred_setTheory pairTheory dep_rewrite arithmeticTheory listTheory
      alistTheory rich_listTheory combinTheory gol_rulesTheory
      integerTheory intLib gol_simTheory gol_lemmasTheory;
 
-val _ = new_theory "gol_mod_step";
+val _ = new_theory "gol_io_step";
 
 Overload LLOOKUP = “λl n. oEL n l”;
 Overload "U" = “BIGUNION”;
@@ -24,8 +24,8 @@ Datatype:
        assert_content : (int # int) set |>
 End
 
-Definition mod_step_def:
-  mod_step c s1 s3 ⇔
+Definition io_step_def:
+  io_step c s1 s3 ⇔
     ∃s2.
       infl s1 ⊆ c.area ∧
       step s1 = s2 ∧
@@ -33,25 +33,25 @@ Definition mod_step_def:
       s3 = c.insertions ∪ (s2 DIFF c.deletions)
 End
 
-Theorem mod_step_univ:
+Theorem io_step_univ:
   c.area = UNIV ∧ c.insertions = EMPTY ∧ c.deletions = EMPTY
   ⇒
-  (mod_step c s1 s2
+  (io_step c s1 s2
    ⇔
    step s1 = s2 ∧
    s2 ∩ c.assert_area = c.assert_content)
 Proof
-  gvs [mod_step_def] \\ metis_tac []
+  gvs [io_step_def] \\ metis_tac []
 QED
 
-Definition mod_steps_def:
-  mod_steps 0 c n s1 s2 = (s1 = s2) ∧
-  mod_steps (SUC k) c n s1 s3 =
-     ∃s2. mod_step (c n) s1 s2 ∧ mod_steps k c (n+1:num) s2 s3
+Definition io_steps_def:
+  io_steps 0 c n s1 s2 = (s1 = s2) ∧
+  io_steps (SUC k) c n s1 s3 =
+     ∃s2. io_step (c n) s1 s2 ∧ io_steps k c (n+1:num) s2 s3
 End
 
 Definition run_to_def:
-  run_to k c s t ⇔ mod_steps k c 0 s t
+  run_to k c s t ⇔ io_steps k c 0 s t
 End
 
 Definition run_def:
@@ -86,21 +86,21 @@ Definition join_def:
            assert_content := (c1 n).assert_content ∪ (c2 n).assert_content |>
 End
 
-Theorem mod_steps_compose:
+Theorem io_steps_compose:
   ∀c1 c2 k n s1 s2 t1 t2.
     disjoint_mods c1 c2 ∧
     mods_wf c1 ∧
     mods_wf c2 ∧
-    mod_steps k c1 n s1 t1 ∧
-    mod_steps k c2 n s2 t2 ⇒
-    mod_steps k (join c1 c2) n (s1 ∪ s2) (t1 ∪ t2)
+    io_steps k c1 n s1 t1 ∧
+    io_steps k c2 n s2 t2 ⇒
+    io_steps k (join c1 c2) n (s1 ∪ s2) (t1 ∪ t2)
 Proof
-  gen_tac \\ gen_tac \\ Induct \\ gvs [mod_steps_def]
+  gen_tac \\ gen_tac \\ Induct \\ gvs [io_steps_def]
   \\ rpt strip_tac \\ gvs []
   \\ last_x_assum drule_all
   \\ rename [‘_ (u1 ∪ u2) (_ ∪ _)’]
   \\ disch_then $ irule_at Any
-  \\ gvs [mod_step_def,join_def]
+  \\ gvs [io_step_def,join_def]
   \\ gvs [infl_union,mods_wf_def,disjoint_mods_def,disjoint_mod_def]
   \\ rpt $ first_x_assum $ qspec_then ‘n’ assume_tac
   \\ gvs [mod_wf_def]
@@ -122,14 +122,14 @@ Definition join_all_def:
       assert_content := U { (cs i n).assert_content | i ∈ dom } |>
 End
 
-Theorem mod_step_compose_bigunion:
+Theorem io_step_compose_bigunion:
   ∀n cs s t.
     (∀x y. x ∈ dom ∧ y ∈ dom ∧ x ≠ y ⇒ disjoint_mods (cs x) (cs y)) ∧
-    (∀i. i ∈ dom ⇒ mods_wf (cs i) ∧ mod_step (cs i n) (s i) (t i))
+    (∀i. i ∈ dom ⇒ mods_wf (cs i) ∧ io_step (cs i n) (s i) (t i))
     ⇒
-    mod_step (join_all (dom, cs) n) (U { s i | i ∈ dom }) (U { t i | i ∈ dom })
+    io_step (join_all (dom, cs) n) (U { s i | i ∈ dom }) (U { t i | i ∈ dom })
 Proof
-  rw [mod_step_def, join_all_def, infl_bigunion]
+  rw [io_step_def, join_all_def, infl_bigunion]
   >- (rw [BIGUNION_SUBSET] \\ irule SUBSET_BIGUNION_SUBSET_I
     \\ simp [PULL_EXISTS] \\ metis_tac [])
   \\ dep_rewrite.DEP_REWRITE_TAC [infl_compose_bigunion]
@@ -158,16 +158,16 @@ Proof
   \\ metis_tac []
 QED
 
-Theorem mod_steps_compose_bigunion:
+Theorem io_steps_compose_bigunion:
   ∀k cs n s t.
     (∀x y. x ∈ dom ∧ y ∈ dom ∧ x ≠ y ⇒ disjoint_mods (cs x) (cs y)) ∧
-    (∀i. i ∈ dom ⇒ mods_wf (cs i) ∧ mod_steps k (cs i) n (s i) (t i))
+    (∀i. i ∈ dom ⇒ mods_wf (cs i) ∧ io_steps k (cs i) n (s i) (t i))
     ⇒
-    mod_steps k (join_all (dom, cs)) n (U { s i | i ∈ dom }) (U { t i | i ∈ dom })
+    io_steps k (join_all (dom, cs)) n (U { s i | i ∈ dom }) (U { t i | i ∈ dom })
 Proof
-  Induct \\ gvs [mod_steps_def]
+  Induct \\ gvs [io_steps_def]
   >- (simp [Once EXTENSION, Once EXTENSION] \\ metis_tac [])
-  \\ metis_tac [mod_step_compose_bigunion]
+  \\ metis_tac [io_step_compose_bigunion]
 QED
 
 Theorem run_compose_bigunion:
@@ -178,8 +178,8 @@ Theorem run_compose_bigunion:
     run (join_all (dom, cs)) (U { s i | i ∈ dom })
 Proof
   rw [run_def, run_to_def]
-  \\ `∀i. i ∈ dom ⇒ ∃t. mod_steps k (cs i) 0 (s i) t` by metis_tac []
-  \\ metis_tac [mod_steps_compose_bigunion]
+  \\ `∀i. i ∈ dom ⇒ ∃t. io_steps k (cs i) 0 (s i) t` by metis_tac []
+  \\ metis_tac [io_steps_compose_bigunion]
 QED
 
 Definition empty_mod_def:
@@ -226,18 +226,18 @@ End
 
 Theorem to_assert:
   ∀k n s t.
-    mod_steps k c n s t ∧
+    io_steps k c n s t ∧
     can_assert p c
     ⇒
-    mod_steps k (assert p c) n s t
+    io_steps k (assert p c) n s t
 Proof
   Induct
-  \\ gvs [mod_steps_def,PULL_EXISTS]
+  \\ gvs [io_steps_def,PULL_EXISTS]
   \\ rpt strip_tac \\ gvs []
   \\ last_x_assum $ drule_then $ irule_at Any
   \\ gvs [can_assert_def]
   \\ first_x_assum $ qspec_then ‘n’ assume_tac
-  \\ gvs [mod_step_def,assert_def,assert_mod_def]
+  \\ gvs [io_step_def,assert_def,assert_mod_def]
   \\ IF_CASES_TAC \\ gvs []
   \\ gvs [EXTENSION,SUBSET_DEF]
   \\ metis_tac []
@@ -275,18 +275,18 @@ End
 
 Theorem to_del_io:
   ∀k n s t.
-    mod_steps k c n s t ∧
+    io_steps k c n s t ∧
     can_assert p c
     ⇒
-    mod_steps k (del_io p c) n s t
+    io_steps k (del_io p c) n s t
 Proof
   Induct
-  \\ gvs [mod_steps_def,PULL_EXISTS]
+  \\ gvs [io_steps_def,PULL_EXISTS]
   \\ rpt strip_tac \\ gvs []
   \\ last_x_assum $ drule_then $ irule_at Any
   \\ gvs [can_assert_def]
   \\ first_x_assum $ qspec_then ‘n’ assume_tac
-  \\ gvs [mod_step_def,del_io_def,del_io_mod_def]
+  \\ gvs [io_step_def,del_io_def,del_io_mod_def]
   \\ IF_CASES_TAC \\ gvs []
   \\ gvs [EXTENSION,SUBSET_DEF]
   \\ metis_tac []
@@ -322,19 +322,19 @@ Definition can_clear_def:
         (c n).assert_content = (c n).insertions
 End
 
-Theorem mod_steps_clear_mods:
+Theorem io_steps_clear_mods:
   ∀k c n s t.
-    mod_steps k c n s t ∧
+    io_steps k c n s t ∧
     can_clear c
     ⇒
-    mod_steps k (clear_mods c) n s t
+    io_steps k (clear_mods c) n s t
 Proof
   Induct
-  \\ gvs [mod_steps_def,PULL_EXISTS]
+  \\ gvs [io_steps_def,PULL_EXISTS]
   \\ rpt strip_tac \\ gvs []
   \\ last_x_assum $ drule_then $ irule_at Any
   \\ gvs [can_assert_def]
-  \\ gvs [mod_step_def,can_clear_def,clear_mods_def,clear_mod_def]
+  \\ gvs [io_step_def,can_clear_def,clear_mods_def,clear_mod_def]
   \\ gvs [EXTENSION,SUBSET_DEF]
   \\ metis_tac []
 QED
@@ -348,7 +348,7 @@ Theorem run_clear_mods:
 Proof
   rw [run_def,run_to_def]
   \\ last_x_assum $ qspec_then ‘k’ strip_assume_tac
-  \\ drule_all mod_steps_clear_mods
+  \\ drule_all io_steps_clear_mods
   \\ disch_then $ irule_at Any
 QED
 
